

9.8 Steepest descent Method in ℓ_∞ -norm

$$\Delta x = \argmin_d \nabla f(x)^T d, \quad \|d\|_\infty \leq 1$$

$$\rightarrow \Delta x = \text{Sign}(\nabla f(x))$$

(10.1) Nonsingularity of the KKT matrix

(a)

$$\checkmark \textcircled{1} \iff \textcircled{2}$$

$$N(p) \cap N(A) = \{0\} \Rightarrow N(A) \perp \text{null}(P) \quad x^T P x > 0$$

$$\Leftrightarrow Ax=0 \Rightarrow x^T P x > 0$$

$$\checkmark \textcircled{2} \iff \textcircled{3}$$

$$F = \text{basis of } N(A) \rightarrow x = Fz, \quad z \in \mathbb{R}^{n \times (n-p)}$$

$$x^T P x = z^T \underbrace{F^T P F}_{P^*} z > 0$$

$$\checkmark \textcircled{2} \iff \textcircled{4}$$

$$P + A^T Q A > 0 \text{ for some } Q \geq 0$$

$$x^T P x + x^T A^T Q A x = x^T P x + (Ax)^T Q (Ax) = x^T p x > 0$$

$$(Ax=0 \rightarrow x^T P x > 0) \iff P + A^T Q A > 0 \text{ for some } Q \geq 0$$



(b) $\begin{bmatrix} P & A^T \\ A & 0 \end{bmatrix}$ has exactly n positive, p negative eigen V
(if (a) holds)

$$P + A^T A > 0. \quad R^T (P + A^T A) R = I$$

$$AR = U \Sigma V_1^T, \quad V = \begin{bmatrix} V_1 & V_2 \end{bmatrix}, \quad S = \begin{bmatrix} \Sigma & 0 \\ 0 & 0 \end{bmatrix} \begin{matrix} n \\ p \end{matrix}$$

$$V^T R^T (P + A^T A) R V = V^T R^T P R V + S^T S = I$$

$$V^T R^T P R V = I - S^T S = \text{diag}(\underbrace{1 - \sigma_1^2, 1 - \sigma_2^2, \dots, 1}_{p}, \dots, 1) = \Lambda$$

$$\begin{bmatrix} V^T R^T & 0 \\ 0 & U^T \end{bmatrix} \begin{bmatrix} P & A^T \\ A & 0 \end{bmatrix} \begin{bmatrix} R V & 0 \\ 0 & U \end{bmatrix} = \begin{bmatrix} \Lambda & S^T \\ S & 0 \end{bmatrix} \begin{matrix} n \\ p \end{matrix}$$

$$\begin{bmatrix} \underbrace{\Lambda}_{p} & 0 & \Sigma \\ 0 & \underbrace{1}_{n-p} & 0 \\ \Sigma & 0 & 0 \end{bmatrix} \begin{matrix} p \\ n-p \\ p \end{matrix}$$

$\hookrightarrow M' = P^T M P, \quad (P : \text{permutation matrix})$

$$\left(\begin{bmatrix} 1 - \sigma_1^2 & \sigma_1 \\ \sigma_1 & 0 \end{bmatrix} \quad \square \quad \square \quad \square \quad \dots \right)$$

\hookrightarrow 합동변환

(11.13) self-concordance and negative entropy

$$(a) \quad f'(x) = 1 + \log x, \quad f''(x) = \frac{1}{x}, \quad f'''(x) = -\frac{1}{x^2}$$

$$\left| -\frac{1}{x^2} \right| \leq 2 \left(\frac{1}{x} \right)^{\frac{3}{2}} \leftarrow \text{False}$$

$$(b) \quad f'(x) = t \log x + t - \frac{1}{x}$$

$$f''(x) = \frac{t}{x} + \frac{1}{x^2}, \quad f'''(x) = -\frac{t}{x^2} - \frac{2}{x^3}$$

$$\left| -\frac{t}{x^2} - \frac{2}{x^3} \right| \leq 2 \left(\frac{t}{x} + \frac{1}{x^2} \right)^{\frac{3}{2}}$$

implementing simple calculus ...

True!